enable match checking

pulse/lib/steel/pulse/Pulse.Checker.fst
@@ -511,29 +511,28 @@ let rec check' : bool -> check_t =
     | Tm_While _ ->
       While.check_while g t pre pre_typing post_hint (check' true)
 
-    // | Tm_Match {sc;returns_=post_match;brs} ->
-    //   // TODO : dedup
-    //   let post =
-    //     match post_match, post_hint with
-    //     | None, Some p -> p
-    //     | Some p, None ->
-    //       Checker.Common.intro_post_hint g None p
-    //     | Some p, Some q ->
-    //       Pulse.Typing.Env.fail g (Some t.range)
-    //         (Printf.sprintf
-    //            "Multiple annotated postconditions---remove one of them.\n\
-    //             The context expects the postcondition %s,\n\
-    //             but this conditional was annotated with postcondition %s"
-    //             (P.term_to_string (q <: post_hint_t).post)
-    //             (P.term_to_string p))
-    //     | _, _ ->
-    //       Pulse.Typing.Env.fail g (Some t.range)
-    //         (Printf.sprintf
-    //            "Pulse cannot yet infer a postcondition for a non-tail conditional statement;\n\
-    //             Either annotate this `if` with `returns` clause; or rewrite your code to use a tail conditional")
-    //   in
-    //   let (| t, c, d |) = Match.check_match g sc brs pre pre_typing post (check' true) in
-    //   ( (| t, c, d |) <: checker_result_t g pre post_hint)
+    | Tm_Match {sc;returns_=post_match;brs} ->
+      // TODO : dedup
+      let post =
+        match post_match, post_hint with
+        | None, Some p -> p
+        | Some p, None ->
+          Checker.Common.intro_post_hint g None p
+        | Some p, Some q ->
+          Pulse.Typing.Env.fail g (Some t.range)
+            (Printf.sprintf
+               "Multiple annotated postconditions---remove one of them.\n\
+                The context expects the postcondition %s,\n\
+                but this conditional was annotated with postcondition %s"
+                (P.term_to_string (q <: post_hint_t).post)
+                (P.term_to_string p))
+        | _, _ ->
+          Pulse.Typing.Env.fail g (Some t.range)
+            (Printf.sprintf
+               "Pulse cannot yet infer a postcondition for a non-tail conditional statement;\n\
+                Either annotate this `if` with `returns` clause; or rewrite your code to use a tail conditional")
+      in
+      Match.check_match g sc brs pre pre_typing post (check' true)
 
     | Tm_ProofHintWithBinders _ ->
       Pulse.Checker.AssertWithBinders.check g t pre pre_typing post_hint (check' true)
