pulse/lib/steel/pulse/Pulse.Checker.Match.fsti
@@ -6,12 +6,12 @@ open Pulse.Syntax
 open Pulse.Typing
 open Pulse.Checker.Common
 
-// val check_match
-//         (g:env)
-//         (sc:term)
-//         (brs:list branch)
-//         (pre:term)
-//         (pre_typing: tot_typing g pre tm_vprop)
-//         (post_hint:post_hint_for_env g)
-//         (check:check_t)
-//   : T.Tac (checker_result_t g pre (Some post_hint))
+val check_match
+        (g:env)
+        (sc:term)
+        (brs:list branch)
+        (pre:term)
+        (pre_typing: tot_typing g pre tm_vprop)
+        (post_hint:post_hint_for_env g)
+        (check:check_t)
+  : T.Tac (checker_result_t g pre (Some post_hint))
